theories/Fixpoints.v
@@ -1,0 +1,155 @@
+Section Fixpoints.
+
+  (* Propositional analogues to definitions from above. *)
+
+  Definition PSet (A : Type) := A -> Prop.
+
+  Definition In {A} (a : A) (e : PSet A) : Prop := e a.
+  Notation "x '∈' e" := (In x e) (at level 60).
+
+  Definition Subset {A} (e1 e2 : PSet A) : Prop :=
+    forall x, x ∈ e1 -> x ∈ e2.
+
+  Notation "s1 ⊆ s2" := (Subset s1 s2) (at level 60).
+
+  Context {U : Type}. (* The universal set, i.e. our domain of discourse. *)
+  Variable F : (PSet U) -> PSet U. (* Our generating function--
+  takes a set of Us and builds a new set.*)
+
+  (* A generator function is monotone if it preserves the subset
+  relation on its argument. *)
+  Definition Monotone_F : Prop :=
+    forall (S S' : PSet U),
+      S ⊆ S' -> F S ⊆ F S'.
+
+  Definition FClosed (S : PSet U) : Prop := F S ⊆ S.
+
+  Definition FConsistent (S : PSet U) : Prop := S ⊆ F S.
+
+  Definition FixedPoint (S : PSet U) : Prop :=
+    S ⊆ F S /\ F S ⊆ S.
+
+  (* The least fixed point of a monotone generator function exists,
+   and it is the intersection of all F-closed sets. *)
+  Definition LFP : PSet U :=
+    fun a => forall S, FClosed S -> S a.
+
+  (* The greatest fixed point of a generator function exists,
+   and it is the union of all F-consistent sets. *)
+  Definition GFP : PSet U :=
+    fun a => exists S, FConsistent S /\ S a.
+
+  Lemma GFP_is_FConsistent
+    : Monotone_F -> FConsistent GFP.
+  Proof.
+    intros F_Monotone.
+    unfold FConsistent.
+    intros ? ?.
+    (* By the definition of GFP, there must be some F-consistent set, X, that contains x *)
+    destruct H as [X [? ?] ].
+    (* Since X is F-consistent, by definition x is a member of F X. *)
+    apply H in H0.
+    (* We have now established that F X ⊆ F GFP: *)
+    revert x H0; fold (Subset (F X) (F GFP)).
+    (* Since F is monotone, it suffices to show that X ⊆ GFP *)
+    eapply F_Monotone.
+    (* To show X ⊆ GFP, we just need to show that every x in X is in GFP *)
+    intros ? ?.
+    (* By definition, x is an element of GFP if it is a member of an
+    F-consistent set. By assumption, x is in X and F is F-consistent,
+    so we're done!*)
+    unfold In, GFP.
+    eexists X.
+    eauto.
+  Qed.
+
+  Lemma GFP_is_FClosed
+    : Monotone_F -> FClosed GFP.
+  Proof.
+    intros F_Monotone ? ?.
+    (* By our previous lemma, we know that GFP ⊆ F GFP. By monotonicity of
+       F, F GFP ⊆ F (F GFP). *)
+    assert (F GFP ⊆ F (F GFP)).
+    { apply F_Monotone.
+      apply GFP_is_FConsistent.
+      eassumption. }
+    (* By definition, this means F GFP is F-consistent. *)
+    assert (FConsistent (F GFP)).
+    { intros ? ?.
+      apply H0.
+      assumption. }
+    (* Since F is a member of an F-consistent set, it must be a member
+    of GFP.*)
+    unfold In, GFP.
+    exists (F GFP).
+    eauto.
+  Qed.
+
+  Theorem GFP_is_FixedPoint
+    : Monotone_F -> FixedPoint GFP.
+  Proof.
+    intro F_Monotone.
+    unfold FixedPoint.
+    split.
+    - apply GFP_is_FConsistent; eauto.
+    - apply GFP_is_FClosed; eauto.
+  Qed.
+
+  Theorem LFP_is_FClosed
+    : Monotone_F -> FClosed LFP.
+  Proof.
+    intro F_Monotone.
+    unfold FClosed; intros ? ? ? ?.
+    apply H0.
+    revert x H.
+    eapply F_Monotone.
+    unfold LFP; intros ? ?.
+    apply H.
+    apply H0.
+  Qed.
+
+  Theorem LFP_is_FConsistent
+    : Monotone_F -> FConsistent LFP.
+  Proof.
+    intro F_Monotone.
+    unfold FClosed; intros ? ?.
+    assert (F (F LFP) ⊆ F LFP).
+    { apply F_Monotone.
+      apply LFP_is_FClosed.
+      eassumption. }
+    (* By definition, this means F LFP is F-closed. *)
+    assert (FClosed (F LFP)).
+    { intros ? ?.
+      apply H0.
+      assumption. }
+    (* Since F is a member of every F-closed set, it must be a member
+    of the F-closed set (F LFP) .*)
+    eapply H.
+    apply H1.
+  Qed.
+
+  Theorem LFP_is_FixedPoint
+    : Monotone_F -> FixedPoint LFP.
+  Proof.
+    intro F_Monotone.
+    unfold FixedPoint.
+    split.
+    - apply LFP_is_FConsistent; eauto.
+    - apply LFP_is_FClosed; eauto.
+  Qed.
+
+  Lemma Ind
+    : forall (Ind : PSet U),
+      FClosed Ind -> forall a, LFP a -> Ind a.
+  Proof.
+    unfold LFP, FClosed; intros; eapply H0; eauto.
+  Qed.
+
+  Lemma CoInd
+    : forall (Ind : PSet U),
+      FConsistent Ind -> forall a, Ind a -> GFP a.
+  Proof.
+    unfold GFP, FConsistent; intros; eauto.
+  Qed.
+
+End Fixpoints.
